bedrock2/src/bedrock2/Scalars.v
@@ -312,13 +312,7 @@ Section Scalars.
     load access_size.four m a = Some (word.of_Z (LittleEndian.combine _ (HList.tuple.of_list bs))).
   Proof. eapply load_four_bytes_of_sep_at; try eapply H; blia. Qed.
 
-  (*
-  Lemma store_four_of_sep addr (oldvalue : word32) (value : word) R m (post:_->Prop)
-    (Hsep : sep (scalar32 addr oldvalue) R m)
-    (Hpost : forall m, sep (scalar32 addr (word.of_Z (word.unsigned value))) R m -> post m)
-    : exists m1, Memory.store Syntax.access_size.four m addr value = Some m1 /\ post m1.
-  Proof.
-  *)
+  Add Ring wring : Properties.word.ring_theory.
 
   Lemma array_store_four_of_sep (addr addr' : word) n (oldvalues : list word) (value : word) size R m (post:_->Prop) (_ : addr' = word.add addr (word.of_Z ((word.unsigned size) * (Z.of_nat n))))
     (Hsep : sep (array scalar32 size addr oldvalues) R m)
@@ -326,9 +320,7 @@ Section Scalars.
     (Hpost : forall m, sep (array scalar32 size addr (upd oldvalues n (truncate_word access_size.four value))) R m -> post m)
     : exists m1, Memory.store Syntax.access_size.four m addr' value = Some m1 /\ post m1.
   Proof.
-    assert (forall l, (n < length l)%nat -> l = firstn n l ++ ((nth n l (word.of_Z 0))::nil) ++ skipn (S n) l).
-    { intros; rewrite <-Nat.add_1_l, <-skipn_skipn, <-firstn_skipn_nth, firstn_skipn, firstn_skipn; auto. }
-    rewrite (H1 oldvalues H0) in Hsep.
+    rewrite <-(firstn_nth_skipn _ _ oldvalues (word.of_Z 0) H0) in Hsep.
     do 2 seprewrite_in (array_append scalar32 size) Hsep.
     seprewrite_in (array_cons scalar32 size) Hsep.
     seprewrite_in (array_nil scalar32 size) Hsep.
@@ -345,7 +337,130 @@ Section Scalars.
     cbn[length Nat.add] in *.
     ecancel_assumption.
   Qed.
+
+  Lemma array_store_four_of_sep_32bit (addr addr' : word) n (oldvalues : list word) (value : word) size R m (post:_->Prop) (_ : addr' = word.add addr (word.of_Z ((word.unsigned size) * (Z.of_nat n))))
+    (W32: width = 32)
+    (Hsep : sep (array scalar32 size addr oldvalues) R m)
+    (_ : (n < length oldvalues)%nat)
+    (Hpost : forall m, sep (array scalar32 size addr (upd oldvalues n value)) R m -> post m)
+    : exists m1, Memory.store Syntax.access_size.four m addr' value = Some m1 /\ post m1.
+  Proof.
+    eapply array_store_four_of_sep; eauto.
+    rewrite truncate_word_nop_32bit; assumption.
+  Qed.
+
+  Lemma array_store_four_of_sep'(addr addr' : word) (oldvalues : list word) (value : word) size R m (post:_->Prop)
+    (Hsep : sep (array scalar32 size addr oldvalues) R m)
+    (_ : 0 < word.unsigned size)
+    (_ : let offset := word.unsigned (word.sub addr' addr) in
+         (Z.modulo offset (word.unsigned size) = 0) /\
+         (let n := Z.to_nat (offset / word.unsigned size) in (n < List.length oldvalues)%nat /\
+    (forall m, sep (array scalar32 size addr (upd oldvalues n (truncate_word access_size.four value))) R m -> post m)))
+    : exists m1, Memory.store Syntax.access_size.four m addr' value = Some m1 /\ post m1.
+  Proof.
+    destruct H0; destruct H1.
+    eapply array_store_four_of_sep; eauto.
+    rewrite Z2Nat.id by (apply Z.div_pos; [apply word.unsigned_range | blia]).
+    rewrite <- Z_div_exact_2; [| blia| auto].
+    rewrite word.of_Z_unsigned.
+    ring.
+  Qed.
+
+  Lemma array_store_four_of_sep_32bit'(addr addr' : word) (oldvalues : list word) (value : word) size R m (post:_->Prop)
+    (W32 : width = 32) 
+    (Hsep : sep (array scalar32 size addr oldvalues) R m)
+    (_ : 0 < word.unsigned size)
+    (_ : let offset := word.unsigned (word.sub addr' addr) in
+         (Z.modulo offset (word.unsigned size) = 0) /\
+         (let n := Z.to_nat (offset / word.unsigned size) in (n < List.length oldvalues)%nat /\
+    (forall m, sep (array scalar32 size addr (upd oldvalues n value)) R m -> post m)))
+    : exists m1, Memory.store Syntax.access_size.four m addr' value = Some m1 /\ post m1.
+   Proof.
+     eapply array_store_four_of_sep'; eauto.
+     rewrite truncate_word_nop_32bit; assumption.
+   Qed.
+
+  Lemma array_load_four_of_sep addr addr' n (values : list word) size R m
+    (Hsep : (sep (array scalar32 size addr values) R m))
+    (_ : addr' = (word.add addr (word.of_Z (word.unsigned size * Z.of_nat n))))
+    (_ : (n < length values)%nat) :
+    Memory.load Syntax.access_size.four m addr' =
+    Some (truncate_word Syntax.access_size.four (nth n values (word.of_Z 0))).
+  Proof.
+    rewrite <-(firstn_nth_skipn _ _ values (word.of_Z 0) H0) in Hsep.
+    do 2 seprewrite_in (array_append scalar32 size) Hsep.
+    seprewrite_in (array_cons scalar32 size) Hsep.
+    seprewrite_in (array_nil scalar32 size) Hsep.
+    rewrite firstn_length, min_l, <-H in Hsep by blia.
+    erewrite <-load_four_of_sep; [|ecancel_assumption].
+    reflexivity.
+  Qed.
+
+  Lemma array_load_four_of_sep_32bit addr addr' n (values : list word) size R m
+    (W32: width = 32)
+    (Hsep : (sep (array scalar32 size addr values) R m))
+    (_ : addr' = (word.add addr (word.of_Z (word.unsigned size * Z.of_nat n))))
+    (_ : (n < length values)%nat) :
+    Memory.load Syntax.access_size.four m addr' = Some (nth n values (word.of_Z 0)).
+  Proof.
+    erewrite array_load_four_of_sep; eauto.
+    rewrite truncate_word_nop_32bit; auto.
+  Qed.
+
+  Lemma array_load_four_of_sep' (addr addr': word) (values : list word) size R m
+    (Hsep : sep (array scalar32 size addr values) R m)
+    (_ : 0 < word.unsigned size)
+    : let offset := word.unsigned (word.sub addr' addr) in
+      (Z.modulo offset (word.unsigned size) = 0) ->
+      (let n := Z.to_nat (offset / word.unsigned size) in (n < List.length values)%nat ->
+      Memory.load Syntax.access_size.four m addr' =
+      Some (truncate_word Syntax.access_size.four (nth n values (word.of_Z 0)))).
+  Proof.
+    intros.
+    erewrite array_load_four_of_sep; eauto.
+    subst offset n.
+    rewrite Z2Nat.id by (apply Z.div_pos; [apply word.unsigned_range | blia]).
+    rewrite <- Z_div_exact_2; [| blia| auto].
+    rewrite word.of_Z_unsigned.
+    ring.
+  Qed.
   (*
+  Lemma array_load_four_of_sep'' (addr addr': word) (values : list word) size R m
+    (Hsep : sep (array scalar32 size addr values) R m)
+    (_ : 0 < word.unsigned size)
+    (_ : word.unsigned (word.sub addr' addr) mod (word.unsigned size) = 0)
+    (_ : word.unsigned (word.sub addr' addr) < word.unsigned size * Z.of_nat (List.length values)) :
+    let n := Z.to_nat (word.unsigned (word.sub addr' addr) / word.unsigned size) in
+    Memory.load Syntax.access_size.four m addr' =
+    Some (truncate_word Syntax.access_size.four (nth n values (word.of_Z 0))).
+    *)
+
+  Lemma array_load_four_of_sep_32bit' (addr addr': word) (values : list word) size R m
+    (W32: width = 32)
+    (Hsep : sep (array scalar32 size addr values) R m)
+    (_ : 0 < word.unsigned size)
+    : let offset := word.unsigned (word.sub addr' addr) in
+      (Z.modulo offset (word.unsigned size) = 0) ->
+      (let n := Z.to_nat (offset / word.unsigned size) in (n < List.length values)%nat ->
+      Memory.load Syntax.access_size.four m addr' =
+      Some (nth n values (word.of_Z 0))).
+  Proof.
+    intros.
+    erewrite array_load_four_of_sep'; eauto.
+    rewrite truncate_word_nop_32bit; auto.
+  Qed.
+  
+  (*
+Lemma array_store_four_of_sep'(addr addr' : word) (oldvalues : list word) (value : word) size R m (post:_->Prop)
+    (Hsep : sep (array scalar32 size addr oldvalues) R m)
+    (_ : 0 < word.unsigned size)
+    (_ : let offset := word.unsigned (word.sub addr' addr) in
+         (Z.modulo offset (word.unsigned size) = 0) /\
+         (let n := Z.to_nat (offset / word.unsigned size) in (n < List.length oldvalues)%nat /\
+    (forall m, sep (array scalar32 size addr (upd oldvalues n (truncate_word access_size.four value))) R m -> post m)))
+    : exists m1, Memory.store Syntax.access_size.four m addr' value = Some m1 /\ post m1.
+
+
   Lemma array_store_four_of_sep (addr addr' : word) n (oldvalues : list word) (value : word) size R m (post:_->Prop) (_ : addr' = word.add addr (word.of_Z ((word.unsigned size) * (Z.of_nat n))))
     (Hsep : sep (array scalar32 size addr oldvalues) R m)
     (_ : (n < length oldvalues)%nat)
@@ -370,7 +485,8 @@ Section Scalars.
     cbn[length] in *.
     ecancel_assumption.
   Qed.
-*)
+   *)
+  (*
   Lemma array_store_four_of_sep_32bit(W32: width = 32) (addr addr' : word) n (oldvalues : list word) (value : word) size R m (post:_->Prop) (_ : addr' = word.add addr (word.of_Z ((word.unsigned size) * (Z.of_nat n))))
     (Hsep : sep (array scalar32 size addr oldvalues) R m)
     (_ : (n < length oldvalues)%nat)
@@ -417,7 +533,7 @@ Section Scalars.
      eapply (array_store_four_of_sep' (Z.eq_le_incl _ _ (eq_sym W32))); eauto.
      rewrite truncate_word_nop_32bit; auto.
    Qed.
-  (*
+  
   Lemma array_store_four_of_sep' (addr addr' : word) (oldvalues : list word) (value : word) size R m (post:_->Prop)
     (Hsep : sep (array scalar32 size addr oldvalues) R m)
     (_ : let n := Z.to_nat (word.unsigned (word.divu (word.sub addr' addr) size)) in (n < List.length oldvalues)%nat /\
