bedrock2/src/bedrock2Examples/memcpy.v
@@ -1,0 +1,243 @@
+
+Require Import bedrock2.Array bedrock2.Scalars bedrock2.SepLogAddrArith.
+From bedrock2.Map Require Import Separation SeparationLogic.
+Require Import bedrock2.Syntax bedrock2.NotationsInConstr bedrock2.NotationsCustomEntry.
+Import Syntax BinInt String List.ListNotations ZArith.
+From coqutil Require Import Word.Interface Map.Interface.
+Require Import coqutil.Byte coqutil.Z.HexNotation coqutil.Z.Lia.
+Require Import Coq.Strings.Ascii.
+Require Import bedrock2.ZnWords.
+
+
+Local Open Scope string_scope. Local Open Scope Z_scope. Local Open Scope list_scope.
+Local Coercion literal (z : Z) : Syntax.expr := Syntax.expr.literal z.
+Local Coercion var (x : string) : Syntax.expr := Syntax.expr.var x.
+
+Local Coercion name_of_func (f : func) := fst f.
+
+Definition memcpy : func :=
+  let dst := "dst" in
+  let src := "src" in
+  let num := "num" in
+  let i := "i" in
+  ("memcpy", ([dst; src; num], nil: list string, bedrock_func_body:(
+    i = (coq:(4) * num); while (i) {
+      store4(dst + coq:(4) * num - i, load4(src + coq:(4) * num - i));
+      i = (i - coq:(4))
+    }))).
+
+Require bedrock2.WeakestPrecondition.
+Require Import bedrock2.Semantics bedrock2.FE310CSemantics.
+Require Import coqutil.Map.Interface coqutil.Word.LittleEndian coqutil.Word.Interface.
+
+Require bedrock2.WeakestPreconditionProperties.
+From coqutil.Tactics Require Import letexists eabstract.
+Require Import bedrock2.ProgramLogic bedrock2.Scalars.
+Require Import coqutil.Z.Lia coqutil.Word.Properties bedrock2.TailRecursion.
+Require Import coqutil.Tactics.Tactics.
+Section WithParameters.
+  Context {p : FE310CSemantics.parameters}.
+
+  (*Definition entry : Type := string * Semantics.word * (Semantics.word -> mem -> Prop).*)
+  Infix "*" := (sep).  
+  Infix "*" := (sep) : type_scope.
+
+  Local Infix "^+" := word.add  (at level 50, left associativity).
+  Local Infix "^-" := word.sub  (at level 50, left associativity).
+  Local Infix "^*" := word.mul  (at level 50, left associativity).
+  Local Notation "/_" := word.of_Z.      (* smaller angle: squeeze a Z into a word *)
+  Local Notation "\_" := word.unsigned.  (* supposed to be a denotation bracket;
+                                          or bigger angle: let a word fly into the large Z space *)
+  Notation array32 := (array scalar32 (word.of_Z 4)).
+  Notation "l .[[ n |==> xs ]]" := (List.upds l n xs) (left associativity, at level 50).
+
+  Ltac subst_words :=
+    repeat match goal with x := _ : word.rep |- _ => subst x end.
+
+     
+  Ltac upds_simpl_step :=
+     match goal with
+     | |- context [ ?l.[[?i |==> ?vs]].[[?j |==> ?vs']] ] =>
+       rewrite <- List.upds_app' by (try reflexivity; ZnWords)
+     | H : context [ ?l.[[?i |==> ?vs]].[[?j |==> ?vs']] ] |- _ =>
+       rewrite <- List.upds_app' in H by (try reflexivity; ZnWords)
+     end.
+   Ltac upds_simpl := unfold List.upd in *; repeat upds_simpl_step.
+
+   Ltac simpl_list_length_exprs ::= rewrite ?List.length_skipn, ?List.firstn_length, ?List.app_length, ?List.length_cons, ?List.length_nil, ?List.repeat_length, ?List.upds_length in *.
+
+   Ltac word_Z_unsigned :=
+     match goal with
+     | H: context [\_ (/_ ?z)] |- _ => rewrite (word.unsigned_of_Z z) in H; change (word.wrap z) with z in H
+     | H: context [/_ (\_ ?z)] |- _ => rewrite (word.of_Z_unsigned z) in H
+     | |- context [\_ (/_ ?z)] => rewrite (word.unsigned_of_Z z); change (word.wrap z) with z
+     | |- context [/_ (\_ ?z)] => rewrite (word.of_Z_unsigned z)
+     end.
+
+ Add Ring wring : (Properties.word.ring_theory (word := Semantics.word))
+        (preprocess [autorewrite with rew_word_morphism],
+         morphism (Properties.word.ring_morph (word := Semantics.word)),
+         constants [Properties.word_cst]).
+
+ Global Instance spec_of_memcpy : spec_of "memcpy" :=
+    fun functions => forall src_ptr dst_ptr src dst off1 off2 buf1 buf2 num R m t,
+        src = src_ptr ^+ /_ (4 * Z.of_nat off1) ->
+        dst = dst_ptr ^+ /_ (4 * Z.of_nat off2) ->
+        4 * (Z.of_nat off1 + \_ num) < 2^width ->
+        4 * (Z.of_nat off2 + \_ num) < 2^width ->
+        Z.of_nat off1 + \_ num <= Z.of_nat (List.length buf1) ->
+        Z.of_nat off2 + \_ num <= Z.of_nat (List.length buf2) ->
+        (array32 src_ptr buf1 * array32 dst_ptr buf2 * R) m ->
+        WeakestPrecondition.call functions "memcpy" t m [dst; src; num]
+        (fun t' m' rets => t = t' /\ rets = nil /\ (array32 src_ptr buf1 * array32 dst_ptr (buf2.[[off2 |==> List.firstn (Z.to_nat (\_ num)) (List.skipn off1 buf1)]]) * R) m').
+
+  Global Instance spec_of_memcpy : spec_of "memcpy" :=
+    fun functions => forall src_ptr dst_ptr src dst off1 off2 buf1 buf2 num R m t,
+        let off1 := \_ (src_ptr ^- src) in
+        off
+        let n1 := 
+        
+        src = src_ptr ^+ /_ (4 * Z.of_nat off1) ->
+        dst = dst_ptr ^+ /_ (4 * Z.of_nat off2) ->
+        4 * (Z.of_nat off1 + \_ num) < 2^width ->
+        4 * (Z.of_nat off2 + \_ num) < 2^width ->
+        Z.of_nat off1 + \_ num <= Z.of_nat (List.length buf1) ->
+        Z.of_nat off2 + \_ num <= Z.of_nat (List.length buf2) ->
+        (array32 src_ptr buf1 * array32 dst_ptr buf2 * R) m ->
+        WeakestPrecondition.call functions "memcpy" t m [dst; src; num]
+        (fun t' m' rets => t = t' /\ rets = nil /\ (array32 src_ptr buf1 * array32 dst_ptr (buf2.[[off2 |==> List.firstn (Z.to_nat (\_ num)) (List.skipn off1 buf1)]]) * R) m').
+
+ 
+ (*
+  Global Instance spec_of_memcpy : spec_of "memcpy" :=
+    fun functions => forall src_ptr dst_ptr off1 off2 buf1 buf2 num R m t,
+        4 * (Z.of_nat off1 + \_ num) < 2^width ->
+        4 * (Z.of_nat off2 + \_ num) < 2^width ->
+        Z.of_nat off1 + \_ num <= Z.of_nat (List.length buf1) ->
+        Z.of_nat off2 + \_ num <= Z.of_nat (List.length buf2) ->
+        (array32 src_ptr buf1 * array32 dst_ptr buf2 * R) m ->
+        WeakestPrecondition.call functions "memcpy" t m [dst_ptr ^+ (/_ (4 * Z.of_nat off2)); src_ptr ^+ (/_ (4 * Z.of_nat off1)); num]
+        (fun t' m' rets => t = t' /\ rets = nil /\ (array32 src_ptr buf1 * array32 dst_ptr (buf2.[[off2 |==> List.firstn (Z.to_nat (\_ num)) (List.skipn off1 buf1)]]) * R) m').
+  *)
+  Lemma memcpy_ok : program_logic_goal_for_function! memcpy.
+  Proof.
+    repeat straightline.
+    subst src dst.
+    refine ((TailRecursion.tailrec (HList.polymorphic_list.cons _ HList.polymorphic_list.nil) ("src"::"dst"::"num"::"i"::nil)%list%string (fun V R T M SRC DST NUM I => PrimitivePair.pair.mk (exists j, V = 4 * \_ NUM - 4 * (Z.of_nat j) /\ V = word.unsigned I /\ SRC = src_ptr ^+ (/_ (4 * Z.of_nat off1)) /\ DST = dst_ptr ^+ (/_ (4 * Z.of_nat off2)) /\ NUM = num /\ (array32 src_ptr buf1 * array32 dst_ptr (List.upds buf2 off2 (List.firstn j (List.skipn off1 buf1))) * R) M) (fun t m src dst num i => t = T /\ i = /_ 0 /\ src = SRC /\ dst = DST /\ num = NUM /\ (array32 src_ptr buf1 * array32 dst_ptr (buf2.[[off2|==>List.firstn (Z.to_nat (\_ num)) (List.skipn off1 buf1)]]) * R) m))) _ _ _ _ _ _ _); cbn [reconstruct map.putmany_of_list HList.tuple.to_list
+             HList.hlist.foralls HList.tuple.foralls
+             HList.hlist.existss HList.tuple.existss
+             HList.hlist.apply  HList.tuple.apply
+             HList.hlist
+             
+             (* List.repeat *) Datatypes.length
+             HList.polymorphic_list.repeat HList.polymorphic_list.length
+             PrimitivePair.pair._1 PrimitivePair.pair._2] in *.
+    { repeat straightline. }
+    { eapply (Z.lt_wf 0). }
+    { exists 0%nat.
+      split; [auto| split; [ZnWords| split; [|split]; [| |split]; auto ] ].
+      cbn[List.firstn].
+      rewrite List.upds_nil'.
+      ecancel_assumption. }
+    { repeat straightline.
+      { eexists.
+        split.
+        { repeat straightline.
+          eexists; split; [|reflexivity].
+          erewrite (array_load_four_of_sep_32bit' src_ptr);
+            [reflexivity | reflexivity | ecancel_assumption| ZnWords| ZnWords| ].
+          word_Z_unsigned.
+          ZnWords. }
+        eapply (array_store_four_of_sep_32bit' dst_ptr);
+          [reflexivity| ecancel_assumption | ZnWords|].
+        replace ( \_ (/_ 4)) with 4 by ZnWords.
+        subst_words.
+        split; [ZnWords|split; [ZnWords|] ].
+        repeat straightline.
+        eexists; eexists; split.
+        { exists (S x4).
+          split; [auto| split; [ZnWords| split; [|split]; [| |split]; auto] ].
+          replace (Z.to_nat (\_(src_ptr ^+ /_ (4 * Z.of_nat off1) ^+ (/_ 4 ^* num) ^- x3 ^- src_ptr) / 4)) with (off1 + x4)%nat in H6 by ZnWords.
+          replace (Z.to_nat (\_ (dst_ptr ^+ /_ (4 * Z.of_nat off2) ^+ (/_ 4 ^* num) ^- x3 ^- dst_ptr) / 4)) with (off2 + x4)%nat in H6 by ZnWords.
+          unfold List.upd in H6.
+          rewrite <-List.upds_app' in H6 by (rewrite firstn_length; ZnWords).
+          replace (nth (off1 + x4) buf1 (/_ 0)) with (nth x4 (List.skipn off1 buf1) (/_ 0)) in H6.
+          2:{ rewrite <-(List.firstn_skipn off1 buf1) at 2.
+              rewrite List.app_nth2, List.firstn_length, min_l.
+              { f_equal; blia. }
+              { ZnWords. }
+              { rewrite List.firstn_length, min_l by ZnWords.
+                blia. } }
+          rewrite List.firstn_nth in H6 by ZnWords.
+          ecancel_assumption. }
+        split; [ZnWords|auto]. }
+       split; [auto| split; [ZnWords| split; [|split]; [| |split]; auto] ].
+      replace (Z.to_nat (\_ num)) with x4 by ZnWords.
+      ecancel_assumption. }
+    repeat straightline.
+    split; [auto| split; [auto|ecancel_assumption] ].
+  Qed.
+
+  (*
+  
+  Global Instance spec_of_memcpy : spec_of "memcpy" :=
+    fun functions => forall src dst buf buf' num R m t,
+        4 * \_ num < 2^width ->
+         \_ num <= Z.of_nat (List.length buf) ->
+         \_ num <= Z.of_nat (List.length buf') ->
+        (array32 src buf * array32 dst buf' * R) m ->
+        WeakestPrecondition.call functions "memcpy" t m [dst; src; num]
+        (fun t' m' rets => t = t' /\ rets = nil /\ (array32 src buf * array32 dst (buf'.[[0|==>List.firstn (Z.to_nat (\_ num)) buf]]) * R) m').
+
+  
+
+  Lemma memcpy_ok : program_logic_goal_for_function! memcpy.
+  Proof.
+    repeat straightline.
+    refine ((TailRecursion.tailrec (HList.polymorphic_list.cons _ HList.polymorphic_list.nil) ("src"::"dst"::"num"::"i"::nil)%list%string (fun V R T M SRC DST NUM I => PrimitivePair.pair.mk (exists j, V = 4 * \_ NUM - 4 * (Z.of_nat j) /\ V = word.unsigned I /\ SRC = src /\ DST = dst /\ NUM = num /\ (array32 src buf * array32 dst (List.upds buf' 0%nat (List.firstn j buf)) * R) M) (fun t m src dst num i => t = T /\ i = /_ 0 /\ src = SRC /\ dst = DST /\ num = NUM /\ (array32 src buf * array32 dst (buf'.[[0|==>List.firstn (Z.to_nat (\_ num)) buf]]) * R) m))) _ _ _ _ _ _ _); cbn [reconstruct map.putmany_of_list HList.tuple.to_list
+             HList.hlist.foralls HList.tuple.foralls
+             HList.hlist.existss HList.tuple.existss
+             HList.hlist.apply  HList.tuple.apply
+             HList.hlist
+             
+             (* List.repeat *) Datatypes.length
+             HList.polymorphic_list.repeat HList.polymorphic_list.length
+             PrimitivePair.pair._1 PrimitivePair.pair._2] in *.
+    { repeat straightline. }
+    { eapply (Z.lt_wf 0). }
+    { exists 0%nat.
+      split; [auto| split; [ZnWords| split; [|split]; [| |split]; auto ] ].
+      cbn[List.firstn].
+      rewrite List.upds_nil'.
+      ecancel_assumption. }
+    { repeat straightline.
+      { eexists.
+        split.
+        { repeat straightline.
+          eexists; split; [|reflexivity].
+          erewrite (array_load_four_of_sep_32bit' src);
+            [reflexivity | reflexivity | ecancel_assumption| ZnWords | ZnWords| ].
+          replace ( \_ (/_ 4)) with 4 by ZnWords.
+          ZnWords. }
+        eapply (array_store_four_of_sep_32bit' dst);
+          [reflexivity| ecancel_assumption | ZnWords|].
+        replace ( \_ (/_ 4)) with 4 by ZnWords.
+        subst_words.
+        split; [ZnWords|split; [ZnWords|] ].
+        repeat straightline.
+        eexists; eexists; split.
+        { exists (S x4).
+          split; [auto| split; [ZnWords| split; [|split]; [| |split]; auto] ].
+          upds_simpl.
+          replace (Z.to_nat (\_(src ^+ (/_ 4 ^* num) ^- x3 ^- src) / 4)) with x4 in H5 by ZnWords.
+          rewrite List.firstn_nth in H5 by ZnWords.
+          ecancel_assumption. }
+        split; [ZnWords|auto]. }
+      split; [auto| split; [ZnWords| split; [|split]; [| |split]; auto] ].
+      replace (Z.to_nat (\_ num)) with x4 by ZnWords.
+      ecancel_assumption. }
+    repeat straightline.
+    split; [auto| split; [auto|ecancel_assumption] ].
+  Qed.
+*)
+End WithParameters.
